Random proof tweaks.
The proof works on HACL CI, but not on Everest CI.
The proof works on OSX, on Linux (interactive) but not on Linux (batch).

The QI profile shows over-triggering of lemma_LowStar.Monotonic.Buffer.loc_disjoint_includes_r

The hints are replayable on OSX and on HACL* CI, but for some reason,
the build is not identical between Everest regression and HACL* CI.

Calling the "right" instances of the lemma does something. Hopefully it
unblocks the CI this time.

code/streaming/Hacl.Streaming.Functor.fst
@@ -708,11 +708,29 @@ let split_at_last_rest_eq (#index : Type0) (c: block index)
   let sz = rest c i total_len in
   ()
 
+let disjointness #index c (i: index) (p: state' c i) (l: B.loc) (h: HS.mem): Lemma
+  (requires B.(loc_disjoint l (footprint c i h p)))
+  (ensures B.(
+    let s = B.deref h p in
+    let State block_state buf _ _ k' = s in
+    loc_disjoint l (footprint_s c i h s) /\
+    loc_disjoint l (loc_addr_of_buffer buf) /\
+    loc_disjoint l (loc_addr_of_buffer p) /\
+    loc_disjoint l (loc_buffer buf) /\
+    loc_disjoint l (c.state.footprint h block_state) /\
+    loc_disjoint l (optional_footprint #_ #i #c.km #c.key h k')
+  ))
+=
+  let s = B.deref h p in
+  let State block_state buf_ _ _ k' = s in
+  B.(loc_disjoint_includes_r l (footprint_s c i h s) (loc_addr_of_buffer buf_));
+  ()
+
 // This rlimit is a bit crazy, but this proof is not stable. It usually
 // goes through fast, but a high rlimit is a security against regression failures.
 #restart-solver
-#push-options "--z3rlimit 300 --z3cliopt smt.arith.nl=false \
-  --using_facts_from '*,-LowStar.Monotonic.Buffer.unused_in_not_unused_in_disjoint_2,-FStar.Seq.Properties.slice_slice'"
+#push-options "--z3rlimit 600 --z3cliopt smt.arith.nl=false --z3refresh \
+  --using_facts_from '*,-LowStar.Monotonic.Buffer.unused_in_not_unused_in_disjoint_2,-FStar.Seq.Properties.slice_slice'"//,-LowStar.Monotonic.Buffer.loc_disjoint_includes_r '"
 let update_small #index c i t t' p data len =
   [@inline_let] let _ = c.state.invariant_loc_in_footprint #i in
   [@inline_let] let _ = c.key.invariant_loc_in_footprint #i in
@@ -733,9 +751,25 @@ let update_small #index c i t t' p data len =
   let buf1 = B.sub buf 0ul sz in
   let buf2 = B.sub buf sz len in
 
+  let buf_ = buf in
+  let index_ = index in
+  disjointness #index_ c i p B.(loc_buffer data) h00;
+  B.(loc_disjoint_includes_r (loc_buffer data) (footprint c i h00 p) (loc_buffer buf1));
+  B.(loc_disjoint_includes_r (loc_buffer data) (footprint c i h00 p) (loc_buffer buf2));
+  B.(loc_disjoint_includes_r (loc_buffer data) (footprint c i h00 p) (loc_buffer buf2));
+  B.(loc_disjoint_includes_r (loc_addr_of_buffer p) (footprint_s c i h00 s) (loc_buffer buf1));
+  B.(loc_disjoint_includes_r (loc_addr_of_buffer p) (footprint_s c i h00 s) (loc_buffer buf2));
+  B.(loc_disjoint_includes_r (loc_addr_of_buffer p) (footprint_s c i h00 s) (loc_buffer buf_));
+  B.(loc_disjoint_includes_r (loc_addr_of_buffer p) (footprint_s c i h00 s) (loc_addr_of_buffer buf_));
+  B.(loc_disjoint_includes_r (loc_addr_of_buffer p) (footprint_s c i h00 s) (c.state.footprint h00 block_state));
+  B.(loc_disjoint_includes_r (loc_addr_of_buffer p) (footprint_s c i h00 s) (optional_footprint #_ #i #c.km #c.key h00 k'));
+  B.(loc_disjoint_includes_r (c.state.footprint h00 block_state) (loc_buffer buf_) (loc_buffer buf2));
+  B.(loc_disjoint_includes_r (optional_footprint #_ #i #c.km #c.key h00 k') (loc_buffer buf_) (loc_buffer buf2));
+
   B.blit data 0ul buf2 0ul len;
   let h1 = ST.get () in
   assert B.(modifies (loc_buffer buf2) h0 h1);
+  assert B.(modifies (loc_buffer buf_) h0 h1);
   B.modifies_trans (footprint c i h00 p) h00 h0 (footprint c i h00 p) h1;
   split_at_last_rest_eq c i t t' p h00;
   assert(
@@ -744,10 +778,11 @@ let update_small #index c i t t' p data len =
   split_at_last_small c i (G.reveal seen_) (B.as_seq h0 data);
   c.state.frame_invariant (B.loc_buffer buf) block_state h0 h1;
   optional_frame #_ #i #c.km #c.key (B.loc_buffer buf) k' h0 h1;
+  assert (c.state.invariant h0 block_state);
   stateful_frame_preserves_freeable #index #(Block?.state c) #i (B.loc_buffer buf2)
-                                    (State?.block_state s) h0 h1;
-  Seq.lemma_eq_intro (B.as_seq h1 data) (B.as_seq h0 data);
+                                    (State?.block_state s) h00 h1;
   assert(preserves_freeable c i p h00 h1);
+  Seq.lemma_eq_intro (B.as_seq h1 data) (B.as_seq h0 data);
 
   let total_len = add_len c i total_len len in
   [@inline_let]
